examples/new_stack/NewStack0.v
@@ -1,0 +1,91 @@
+Require Import Coqlib.
+Require Import Universe.
+Require Import STS.
+Require Import Behavior.
+Require Import ModSem.
+Require Import Skeleton.
+Require Import PCM.
+Require Import Mem1.
+Require Import TODO TODOYJ.
+
+Set Implicit Arguments.
+
+
+
+
+
+Section PROOF.
+
+  Context `{Σ: GRA.t}.
+  Context `{@GRA.inG memRA Σ}.
+
+(***
+(Replaced asterisk with # because of coq-mode's parsing)
+int pop(struct Node## llref) {
+  if(#llref) {
+    int v = (#llref)->val;
+    struct Node* next = (#llref)->next;
+    free(#llref);
+    (#llref) = next;
+    return v;
+  }
+  return -1;
+}
+***)
+
+  Definition popF: list val -> itree Es val :=
+    fun varg =>
+      `llref: val <- (pargs [Tuntyped] varg)?;;
+      `ll: val    <- (ccall "load" [llref]);;
+      `b: val     <- (ccall "cmp"  [ll; Vnullptr]);;
+      if is_zero b
+      then (
+          '(blk, ofs) <- (parg Tptr ll)?;;
+          let addr_val  := Vptr blk ofs in
+          let addr_next := Vptr blk (ofs + 1) in
+          `v: val    <- (ccall "load"  [addr_val]);;
+          (* `_: val    <- (ccall "debug" [v]);; *)
+          `next: val <- (ccall "load"  [addr_next]);;
+          `_: val    <- (ccall "free"  [addr_val]);;
+          `_: val    <- (ccall "free"  [addr_next]);; (*** change "free"s specification ***)
+          `_: val    <- (ccall "store" [llref; next]);;
+          Ret v
+        )
+      else Ret (Vint (- 1))
+  .
+
+(* struct Node* push(struct Node* ll, int x) { *)
+(*   struct Node* new_node = malloc(sizeof(struct Node)); *)
+(*   new_node->val = x; *)
+(*   new_node->next = ll; *)
+(*   printf("[DEBUG]: "); *)
+(*   print_all(new_node); *)
+(*   return new_node; *)
+(* } *)
+
+  Definition pushF: list val -> itree Es val :=
+    fun varg =>
+      '(node, v)     <- (pargs [Tuntyped; Tuntyped] varg)?;;
+      `_: val        <- (ccall "debug" [v]);;
+      `new_node: val <- (ccall "alloc" [Vint 2]);;
+      addr_v         <- (vadd new_node (Vint 0))?;;
+      addr_next      <- (vadd new_node (Vint 1))?;;
+      `_: val        <- (ccall "store" [addr_v;    v]);;
+      `vret: val     <- (ccall "store" [addr_next; node]);;
+      Ret addr_v
+  .
+
+  Definition StackSem: ModSem.t := {|
+    ModSem.fnsems := [("pop", cfun popF); ("push", cfun pushF)];
+    ModSem.mn := "Stack";
+    ModSem.initial_mr := ε;
+    ModSem.initial_st := tt↑;
+  |}
+  .
+
+  Definition Stack: Mod.t := {|
+    Mod.get_modsem := fun _ => StackSem;
+    Mod.sk := Sk.unit;
+  |}
+  .
+End PROOF.
