examples/new_stack/NewStack1.v
@@ -1,0 +1,95 @@
+Require Import Coqlib.
+Require Import Universe.
+Require Import STS.
+Require Import Behavior.
+Require Import ModSem.
+Require Import Skeleton.
+Require Import PCM.
+Require Import HoareDef OpenDef.
+Require Import Logic.
+Require Import Mem1.
+Require Import TODOYJ.
+
+Set Implicit Arguments.
+
+
+
+
+
+Section PROOF.
+
+  Context `{Σ: GRA.t}.
+  Context `{@GRA.inG memRA Σ}.
+
+  Fixpoint is_list (ll: val) (xs: list val): iProp :=
+    match xs with
+    | [] => (⌜ll = Vnullptr⌝: iProp)%I
+    | xhd :: xtl =>
+      (∃ lhd ltl, ⌜ll = Vptr lhd 0⌝ ** (OwnM ((lhd,0%Z) |-> [xhd; ltl]))
+                             ** is_list ltl xtl: iProp)%I
+    end
+  .
+
+  Definition pop_spec: ftspec unit unit :=
+    (mk_ksimple (fun '(llref, xs) => (
+                     (fun varg o =>
+                        (∃ ll, ⌜varg = [Vptr llref 0%Z]↑⌝ ** OwnM ((llref,0%Z) |-> [ll])
+                                                       ** (is_list ll xs) ** ⌜o = ord_pure 2⌝: iProp)%I),
+                     (fun vret =>
+                        (match xs with
+                         | [] => ⌜vret = (Vint (- 1))↑⌝
+                         | xhd :: xtl => ⌜vret = xhd↑⌝ ** (∃ ll', OwnM ((llref,0%Z) |-> [ll']) ** is_list ll' xtl)
+                         end: iProp)%I)
+    ))).
+
+  Definition push_spec: ftspec unit unit :=
+    (mk_ksimple (fun '(x, xs) => (
+                     (fun varg o => (∃ ll, ⌜varg = [ll; x]↑⌝ ** is_list ll xs ** ⌜o = ord_pure 2⌝)%I),
+                     (fun vret => (∃ ll', is_list ll' (x :: xs) ** ⌜vret = ll'↑⌝)%I)
+    ))).
+
+  Definition StackSbtb: list (gname * kspecbody) :=
+    [("pop", mk_kspecbody pop_spec
+                          (fun args => trigger (kCall "debug" (inr args));;; APCK;;; trigger (Choose _)));
+    ("push",   mk_kspecbody push_spec (fun _ => APCK;;; trigger (Choose _)))
+    ].
+
+  Definition StackStb: list (gname * fspec).
+    eapply (Seal.sealing "stb").
+    let x := constr:(List.map (map_snd (fun ksb => (KModSem.disclose_ksb ksb): fspec)) StackSbtb) in
+    let y := eval cbn in x in
+    eapply y.
+  Defined.
+
+  Definition DebugStb: list (gname * fspec).
+   eapply (Seal.sealing "stb").
+   eapply [("debug", fspec_trivial2)].
+  Defined.
+
+  Definition KStackSem: KModSem.t := {|
+    KModSem.fnsems := StackSbtb;
+    KModSem.mn := "Stack";
+    KModSem.initial_mr := ε;
+    KModSem.initial_st := tt↑;
+  |}
+  .
+
+  Definition SStackSem: SModSem.t := (KModSem.to_tgt) KStackSem.
+
+  Definition StackSem (stb: list (string * fspec)): ModSem.t :=
+    (SModSem.to_tgt stb) SStackSem.
+
+  Definition KStack: KMod.t := {|
+    KMod.get_modsem := fun _ => KStackSem;
+    KMod.sk := Sk.unit;
+  |}
+  .
+
+  Definition SStack: SMod.t := (KMod.to_tgt) KStack.
+
+  Definition Stack (stb: Sk.t -> list (string * fspec)): Mod.t :=
+    SMod.to_tgt stb SStack.
+
+End PROOF.
+Global Hint Unfold StackStb: stb.
+Global Hint Unfold DebugStb: stb.
